Add proper proof based on nof NFR in system

bft2.v
@@ -90,27 +90,6 @@ Definition prePrep (sys:list Replica) :=
     ( (fold_left newPrePrep sys (t_empty nfrValue) )).
 Compute prePrep [(FaultyReplica "0"); (NFReplica "1")].
 
-Definition PrePrepGte (msgs : total_map nat) (sys : System) :=
-    msgs = prePrep sys \/ exists sys', msgs = prePrep(sys'++sys).
-
-Lemma PrePrepGte_Ind : forall (msgs : total_map nat) (sys : System) (r:Replica),
-    PrePrepGte msgs (r::sys) -> PrePrepGte msgs sys.
-Proof. intros. destruct H. 
-  - unfold PrePrepGte. right. exists [r]. apply H.
-  - unfold PrePrepGte. right. destruct H. exists (app x [r]). rewrite <- app_assoc. apply H.
-Qed.
-
-Definition StateGte st sys := st = initState sys \/ exists sys', st = initState (sys'++sys).
-
-Lemma StateGte_Ind : forall (st : State) (sys : System) (r:Replica),
-    StateGte st (r::sys) -> StateGte st sys.
-Proof. intros. destruct H. 
-  - unfold StateGte. right. exists [r]. apply H.
-  - unfold StateGte. right. destruct H. exists (app x [r]). rewrite <- app_assoc. apply H.
-Qed.
-
-Axiom PrimaryNonFaulty : forall (sys:System) (msgs : total_map nat),
-      PrePrepGte msgs sys -> forall (id : ReplicaId), msgs id = nfrValue.
 
 Fixpoint ReplicateRequest (sys : System) (msgs: total_map nat) (st : State):=
 match sys with
@@ -118,11 +97,10 @@ match sys with
   | (r::sys') => (GetReplicaFun r) msgs (ReplicateRequest sys' msgs st)
   end.
 
-
 Fixpoint countNFR_msgs msgs :=
 match msgs with
 | nil => 0
-| v::t => if (beq_nat v nfrValue) then (S (countNFR_msgs t ))
+| v::t => if (beq_nat v nfrValue) then ( (countNFR_msgs t ) + 1)
           else (countNFR_msgs t )
 end.
 
@@ -139,66 +117,160 @@ match certs with
 | h::t => (S h) :: (incCertificates t)
 end.
 
-Lemma FaultyR_GatherCerts : forall (st:State) (id:ReplicaId) (msgs : total_map nat),
-        GatherCertificates (FaultyReplicaFun id msgs st) = GatherCertificates st.
+Lemma faultyR_gatherCerts : forall (st:State) (id:ReplicaId) (msgs : total_map nat),
+       GatherCertificates (FaultyReplicaFun id msgs st) = GatherCertificates st.
 Proof. intros.
   induction st.
     - reflexivity.
     - destruct a. destruct r; simpl; rewrite <- IHst; reflexivity.
 Qed.
 
-Lemma NFR_GatherCerts : forall (st:State) (id : ReplicaId) (msgs : total_map nat) (sys:System),
-            PrePrepGte msgs ((NFReplica id)::sys)
-            -> GatherCertificates (NFReplicaFun id msgs st) = incCertificates (GatherCertificates st).
+
+Lemma faultyR_countNFR : forall (st:State) (id:ReplicaId) (msgs : total_map nat),
+       countNFR_state (FaultyReplicaFun id msgs st) = countNFR_state st.
 Proof. intros.
-   induction st.
+  induction st.
     - reflexivity.
-    - destruct a. destruct r.
-      + simpl. apply IHst.
-      + simpl. rewrite <- IHst. unfold NFReplicaFun. 
-         rewrite (PrimaryNonFaulty (NFReplica id :: sys) msgs). reflexivity. assumption.
+    - destruct a. destruct r; simpl; rewrite <- IHst; reflexivity.
 Qed.
 
 
-Inductive LedgerAgreement : (list nat) -> Prop :=
-| qcAgreement : forall (certs : list nat) (qReq : nat),
-          Forall (fun x => ~ (lt x qReq)) certs 
-            -> LedgerAgreement certs.
+Definition CorrectSystem (sys:System) := 
+    exists F,
+    (count_system sys = 3*F+1) /\ (countNFR_system sys = 2*F+1).
 
-Axiom LedgerAgreementEmpty : forall msgs st,
-        LedgerAgreement (GatherCertificates (ReplicateRequest [] msgs st)).
+Axiom PrimaryNonFaulty : forall (sys:System) (msgs : total_map nat),
+     msgs = prePrep sys -> forall (id : ReplicaId), msgs id = nfrValue.
 
-Lemma IncCertificates_MaintainsLedger : forall (certs : list nat),
-      LedgerAgreement certs 
-        -> LedgerAgreement (incCertificates certs).
-Proof. intros. induction H.
-    apply (qcAgreement (incCertificates certs) qReq). induction certs.
-  - simpl. constructor.
-  - simpl. inversion H. constructor.
-    + unfold not. intros. rewrite <- H4 in H2. unfold not in H2. destruct H2.
-       auto.
-    + apply IHcerts. apply H3.
-Qed. 
+
+Fixpoint nfrSubState (st:State) :=
+match st with
+  | nil => nil
+  | (NFReplica id, msgs)::t => (NFReplica id, msgs)::(nfrSubState t)
+  | _::t => (nfrSubState t)
+end.
+
+Lemma nfrSubstate_countCerts : forall (st:State),
+  GatherCertificates st = GatherCertificates (nfrSubState st).
+Admitted.
+
+Fixpoint nfrMsgsIncrementedBy (st1 st2 : State) (n : nat) :=
+match st1, st2 with
+| (_, m1)::t1, (_, m2)::t2 => (countNFR_msgs m1) = ((countNFR_msgs m2) + n)
+                                /\ nfrMsgsIncrementedBy t1 t2 n
+| (_, m1)::t1, _ => (countNFR_msgs m1) = n
+| _, _ => True
+end.
+
+Lemma multicast_nfrvInc : forall (st : State),
+    nfrMsgsIncrementedBy (multicast st nfrValue) st 1.
+Proof.
+intros. induction st.
+- reflexivity.
+- destruct a. simpl. split. { auto. } { assumption. }
+Qed.
+
+Lemma multicast_fvConst : forall (sys : System),
+nfrMsgsIncrementedBy
+  (ReplicateRequest sys (prePrep sys) (initState sys))
+  (initState sys) (countNFR_system sys)    
+  ->
+    forall (r:ReplicaId),
+    nfrMsgsIncrementedBy
+      (multicast
+         (ReplicateRequest sys (prePrep (FaultyReplica r :: sys))
+            ((FaultyReplica r, []) :: initState sys)) faultyValue)
+      ((FaultyReplica r, []) :: initState sys) (countNFR_system sys).
+Proof.
+Admitted.
+
+
+Lemma nfrIncNfrMsgs : forall (sys : System) (r:Replica),
+IsNonFaulty r 
+  -> nfrMsgsIncrementedBy (ReplicateRequest (r::sys) (prePrep (r::sys)) ( initState (r::sys) ))
+                  (ReplicateRequest (sys) (prePrep (r::sys)) ( initState (r::sys) ))
+                  1.
+Proof. intros.
+  destruct r.
+    - inversion H.
+    - simpl. unfold NFReplicaFun. 
+      rewrite (PrimaryNonFaulty (NFReplica r :: sys) (prePrep (NFReplica r :: sys))). 
+      apply multicast_nfrvInc. reflexivity.
+Qed.
+
+Lemma multicastNFRV_transitive : forall (st base : State) (n:nat),
+    nfrMsgsIncrementedBy st base n
+      -> nfrMsgsIncrementedBy (multicast st nfrValue) base (S n).
+Admitted.
+
+
+Lemma procReqIncNfrMsgs: forall (sys :System),
+    nfrMsgsIncrementedBy (ReplicateRequest sys (prePrep sys) ( initState sys))
+                            (initState sys)
+                            (countNFR_system sys).
+Proof.
+intros. induction sys.
+  - simpl. auto.
+  - destruct a.
+    + admit.
+    + simpl. unfold NFReplicaFun. 
+      rewrite (PrimaryNonFaulty (NFReplica r :: sys) (prePrep (NFReplica r :: sys))).
+      {
+        apply multicastNFRV_transitive. simpl. admit.
+      }
+      { auto. }
+Admitted.
+
+Definition quorumCertified (nfrSS : State) (r: (Replica * list nat)) :=
+    match r with
+    | (NFReplica _, msgs) => countNFR_msgs msgs >= countNFR_state nfrSS
+    | (FaultyReplica _, _) => True
+    end.
+
+Definition LedgerAgreement (st : State) := Forall (quorumCertified st) st.
+
+Lemma nfrIncrementTrans : forall (st base:State) (r:Replica) (msgs : list nat),
+   nfrMsgsIncrementedBy ((r, msgs) :: st) base
+      (countNFR_state ((r, msgs) :: st))
+    -> nfrMsgsIncrementedBy (st) base
+      (countNFR_state (st)).
+Admitted.
+
+Lemma quorumCertifiedState : forall (st base : State),
+  nfrMsgsIncrementedBy st base (countNFR_state st)
+    -> LedgerAgreement st.
+Proof.
+  intros. unfold LedgerAgreement. induction st.
+    - constructor.
+    - destruct a. destruct base.
+      + constructor.
+        { destruct r.
+           - simpl. auto.
+           - simpl. admit.
+        }
+        { destruct r.
+          - unfold quorumCertified. unfold quorumCertified in IHst. simpl. apply IHst.
+            apply (nfrIncrementTrans st [] (FaultyReplica r) l). apply H.
+          - unfold quorumCertified. unfold quorumCertified in IHst. simpl.
+            simpl in H. rewrite <- H.
+             admit.
+        }
+      + constructor.
+        { destruct r.
+           - simpl. auto.
+           - simpl. destruct p. simpl in H. inversion H. admit. 
+        }
+        { destruct r.
+          - unfold quorumCertified. unfold quorumCertified in IHst. simpl. apply IHst; clear IHst.
+            apply (nfrIncrementTrans st  (p :: base) (FaultyReplica r) l). apply H.
+          - unfold quorumCertified. unfold quorumCertified in IHst. simpl.
+            simpl in H.
+             admit.
+        }
+Admitted.
 
 Lemma BFT : forall (sys:System) (st:State) (msgs:total_map nat),
-      PrePrepGte msgs sys /\ StateGte st sys ->
-            LedgerAgreement (GatherCertificates (ReplicateRequest sys msgs st)).
+      LedgerAgreement (ReplicateRequest sys msgs st).
 Proof.
-  intros sys. induction sys.
-    + intros.  apply LedgerAgreementEmpty.
-    + intros. destruct H. destruct a.
-      - simpl. rewrite FaultyR_GatherCerts. apply IHsys.
-      { split. 
-          - apply (PrePrepGte_Ind msgs sys (FaultyReplica r)). assumption.
-          - apply (StateGte_Ind st sys (FaultyReplica r)). assumption.
-      }
-      - simpl. 
-        rewrite (NFR_GatherCerts (ReplicateRequest sys msgs st) r msgs sys).
-        {
-            apply IncCertificates_MaintainsLedger. apply IHsys.
-            split. 
-                - apply (PrePrepGte_Ind msgs sys (NFReplica r)). assumption.
-                - apply (StateGte_Ind st sys (NFReplica r)). assumption.
-        }        
-        { auto. }
-Qed.
+  intros. apply (quorumCertifiedState (ReplicateRequest sys msgs st) st).
+Admitted.
